docs/lib/nat.md
@@ -17,10 +17,10 @@ The iterator for natural numbers:
 
 A simpler case-analysis operation:
 
-    natcase : intersect (i : level) (a : U i) . nat -> a -> (nat -> a) -> a
+    nat_case : intersect (i : level) (a : U i) . nat -> a -> (nat -> a) -> a
 
-    natcase (zero) z s --> z
-    natcase (succ n) z s --> s n
+    nat_case (zero) z s --> z
+    nat_case (succ n) z s --> s n
 
 
 ### Equality
@@ -144,7 +144,7 @@ Strong induction for natural numbers:
     minus : nat -> nat -> nat
 
     minus m (zero) --> m
-    minus m (succ n) --> natcase m zero (fn m' . minus m' n)
+    minus m (succ n) --> nat_case m zero (fn m' . minus m' n)
 
     plus_minus_cancel_l : forall (m n : nat) . m + n - m = n : nat
 
