library/wtype.md
@@ -1,0 +1,41 @@
+open:Wtype
+# `Wtype`
+
+Martin-L&ouml;f's well-founded (or "W") types are a solution to the equation:
+
+    wtype (x : A) . B(x)  ==  exists (x : A) . B(x) -> wtype (x' : A) . B(x')
+
+Martin-L&ouml;f (1984) intended them as constructive ordinals, but
+they can also be used to implement a variety of data structures.  (In
+Istari, datatypes usually provide a more convenient mechanism with
+better canonicity properties.)
+
+    wtype : type:wtype
+          = def:wtype
+
+    wtype_unroll : type:wtype_unroll
+
+    wtype_roll : type:wtype_roll
+
+    wtype_eeqtp : type:wtype_eeqtp
+
+    wind : type:wind
+         =rec= defrec:wind
+
+    wtype_iter : type:wtype_iter
+               = def:wtype_iter
+
+The unroll rewrite for wtype_iter is:
+
+    wtype_iter a b P f m --> f (m #1) (m #2) (fn z . wtype_iter a b P f (m #2 z)) ;
+
+It can be found in the registry as `Wtype.unroll_wtype_iter`.
+
+Induction over W-types employs the `precedes` predicate, wherein
+`precedes A B M N` states that `M` is an immediate prececessor of
+`N`:
+
+    precedes : type:precedes
+             = def:precedes
+
+    precedes_well_founded : type:precedes_well_founded
